Term.v
@@ -4,7 +4,8 @@ Require Import Autosubst.Autosubst.
 Inductive trm :=
   | trm_var (n : var)
   | trm_abs (t : { bind trm })
-  | trm_app (t1 t2 : trm).
+  | trm_app (t1 t2 : trm)
+  | trm_let (t1 : trm) (t2 : { bind trm }).
 
 Instance Ids_trm : Ids trm. derive. Defined.
 Instance Rename_trm : Rename trm. derive. Defined.
@@ -16,13 +17,19 @@ Inductive value : trm -> Prop := val_abs t : value (trm_abs t).
 Inductive cbv : trm -> trm -> Prop :=
   | cbv_appabs t11 v2 :
       value v2 ->
-      cbv (trm_app (trm_abs t11) v2) (t11.[v2/])
+      cbv (trm_app (trm_abs t11) v2) t11.[v2/]
   | cbv_appl t1 t1' t2 :
       cbv t1 t1' ->
       cbv (trm_app t1 t2) (trm_app t1' t2)
   | cbv_appr v1 t2 t2' :
       value v1 ->
       cbv t2 t2' ->
-      cbv (trm_app v1 t2) (trm_app v1 t2').
+      cbv (trm_app v1 t2) (trm_app v1 t2')
+  | cbv_letl t1 t1' t2 :
+      cbv t1 t1' ->
+      cbv (trm_let t1 t2) (trm_let t1' t2)
+  | cbv_let v1 t2 :
+      value v1 ->
+      cbv (trm_let v1 t2) t2.[v1/].
 
 Hint Constructors value cbv.
